Update Submission.thy

homework/06/Submission.thy
@@ -8,13 +8,43 @@ fun ccomp :: "com \<Rightarrow> instr list" where
 "ccomp (c\<^sub>1;;c\<^sub>2) = ccomp c\<^sub>1 @ ccomp c\<^sub>2" |
 "ccomp (IF b THEN c\<^sub>1 ELSE c\<^sub>2) =
   (let cc\<^sub>1 = ccomp c\<^sub>1; cc\<^sub>2 = ccomp c\<^sub>2; cb = bcomp b False (size cc\<^sub>1 + 1)
-   in cb @ cc\<^sub>1 @ JMP (size cc\<^sub>2) # cc\<^sub>2)"
-| "ccomp _ = undefined"
+   in cb @ cc\<^sub>1 @ JMP (size cc\<^sub>2) # cc\<^sub>2)" |
+"ccomp (Loop c b) =
+ (let cc = ccomp c; cb = bcomp b False 1
+  in cc @ cb @ [JMP (-(size cc + size cb + 1))])"
 
 value "ccomp (Loop (''u'' ::= Plus (V ''u'') (N 1)) (Less (N 0) (V ''u'')))"
 
 lemma ccomp_bigstep:
   "(c,s) \<Rightarrow> t \<Longrightarrow> ccomp c \<turnstile> (0,s,stk) \<rightarrow>* (size(ccomp c),t,stk)"
-  sorry
+  proof(induction arbitrary: stk rule: big_step_induct)
+  case (Assign x a s)
+  show ?case by (fastforce simp:fun_upd_def cong: if_cong)
+next
+  case (Seq c1 s1 s2 c2 s3)
+  let ?cc1 = "ccomp c1"  let ?cc2 = "ccomp c2"
+  have "?cc1 @ ?cc2 \<turnstile> (0,s1,stk) \<rightarrow>* (size ?cc1,s2,stk)"
+    using Seq.IH(1) by fastforce
+  moreover
+  have "?cc1 @ ?cc2 \<turnstile> (size ?cc1,s2,stk) \<rightarrow>* (size(?cc1 @ ?cc2),s3,stk)"
+    using Seq.IH(2) by fastforce
+  ultimately show ?case by simp (blast intro: star_trans)
+next
+  case (LoopTrue c s1 s2 b s3)
+  let ?cc = "ccomp c"
+  let ?cb = "bcomp b False 1"
+  let ?cl = "ccomp(Loop c b)"
+  have "?cl \<turnstile> (0,s1,stk) \<rightarrow>* (size ?cc,s2,stk)"
+    by (simp add: LoopTrue.IH(1) exec_appendR)
+  moreover
+  have "?cl \<turnstile> (size ?cc,s2,stk) \<rightarrow>* (size ?cc + size ?cb,s2,stk)"
+    using \<open>bval b s2\<close> by fastforce
+  moreover
+  have "?cl \<turnstile> (size ?cc + size ?cb,s2,stk) \<rightarrow>* (0,s2,stk)"
+    by fastforce
+  moreover
+  have "?cl \<turnstile> (0,s2,stk) \<rightarrow>* (size ?cl,s3,stk)" by(rule LoopTrue.IH(2))
+  ultimately show ?case by(blast intro: star_trans)
+qed fastforce+
 
 end
